Work on percolating the dependent types.

deps/poulet4/lib/P4automata/P4automaton.v
@@ -3,121 +3,120 @@ Require Import Coq.Classes.EquivDec.
 Require Import Coq.micromega.Lia.
 Require Import Compare_dec.
 Require Import Poulet4.Relations.
+Require Import Poulet4.P4automata.Ntuple.
+From Equations Require Import Equations.
 
 Record p4automaton := MkP4Automaton {
   store: Type;
   states: Type;
   size: states -> nat;
-  update: states -> list bool -> store -> store;
+  update: forall (S: states), n_tuple bool (size S) -> store -> store;
   transitions: states -> store -> states + bool;
   cap: forall s, 0 < size s;
 }.
 
-Definition configuration (a: p4automaton) : Type :=
-  (states a + bool) * store a * list bool
-.
+Definition state_ref (a: p4automaton) : Type := states a + bool.
 
-Definition size' (a: p4automaton) (s: a.(states) + bool) : nat :=
-  match s with
-  | inl s => a.(size) s
-  | inr _ => 1
-  end.
+Equations size'
+  (a: p4automaton)
+  (s: state_ref a)
+  : nat := {
+  size' a (inl s) := size a s;
+  size' a (inr _) := 1
+}.
+
+Equations update'
+  (a: p4automaton)
+  (s: state_ref a)
+  (buf: n_tuple bool (size' a s))
+  (st: store a)
+  : store a := {
+  update' a (inl s) buf st := update a s buf st;
+  update' a (inr _) _ st := st
+}.
+
+Equations transitions'
+  (a: p4automaton)
+  (s: state_ref a)
+  (st: store a)
+  : state_ref a := {
+  transitions' a (inl s) st := transitions a s st;
+  transitions' a (inr b) st := inr b
+}.
+
+Lemma cap' (a: p4automaton): forall s, 0 < size' a s.
+Proof.
+  destruct s; auto.
+  rewrite size'_equation_1.
+  apply cap.
+Qed.
+
+Record configuration (a: p4automaton) := MkConfiguration {
+  conf_state: state_ref a;
+  conf_buf_len: nat;
+  conf_buf: n_tuple bool conf_buf_len;
+  conf_buf_sane: conf_buf_len < size' a conf_state;
+  conf_store: store a
+}.
+
+Definition initial_configuration
+  {a: p4automaton}
+  (state: states a)
+  (store: store a)
+:= {|
+  conf_state := inl state;
+  conf_buf_len := 0;
+  conf_buf := tt : n_tuple bool 0;
+  conf_buf_sane := cap a state;
+  conf_store := store
+|}.
+
+Lemma squeeze {n m}: n < m -> m <= n+1 -> n+1 = m.
+Proof.
+  lia.
+Qed.
 
 Definition step
   {a: p4automaton}
   (c: configuration a)
   (b: bool)
-  : configuration a
-:=
-  let '(state, st, buf) := c in
-  let buf' := buf ++ b :: nil in
-  if length buf' == size' a state
-  then
-    match state with
-    | inl state =>
-      let st' := update a state buf' st in
-      let state' := transitions a state st' in
-      (state', st', nil)
-    | inr b =>
-      (inr false, st, nil)
-    end
-  else (state, st, buf')
-.
+  : configuration a :=
+  let buf_padded := n_tuple_app (conf_buf _ c) b in
+  match le_lt_dec (size' a (conf_state _ c)) (conf_buf_len _ c + 1) with
+  | left Hle =>
+    let buf_full := eq_rect _ _ buf_padded _ (squeeze (conf_buf_sane _ c) Hle) in
+    let conf_store' := update' a (conf_state _ c) buf_full (conf_store _ c) in
+    let conf_state' := transitions' a (conf_state _ c) conf_store' in
+    {|
+      conf_state := conf_state';
+      conf_buf := tt : n_tuple bool 0;
+      conf_buf_sane := cap' _ conf_state';
+      conf_store := conf_store';
+    |}
+  | right conf_buf_sane' =>
+    {|
+      conf_state := conf_state _ c;
+      conf_buf := buf_padded;
+      conf_buf_sane := conf_buf_sane';
+      conf_store := conf_store _ c;
+    |}
+  end.
 
-Lemma step_with_space
-  {a: p4automaton}
-  (s: states a)
-  (st: store a)
-  (buf: list bool)
-  (b: bool)
-:
-  length buf + 1 < size a s ->
-  step (inl s, st, buf) b = (inl s, st, buf ++ b :: nil)
-.
-Proof.
-  intros; simpl.
-  destruct (equiv_dec _ _); auto.
-  unfold "===" in e.
-  rewrite app_length in e.
-  simpl length in e.
-  lia.
-Qed.
-
-Definition follow
+Equations follow
   {a: p4automaton}
   (c: configuration a)
   (input: list bool)
-  : configuration a
-:=
-  fold_left step input c
-.
-
-Lemma follow_cons
-  {a: p4automaton}
-  (c: configuration a)
-  (b: bool)
-  (input: list bool)
-:
-  follow c (b :: input) = follow (step c b) input
-.
-Proof.
-  reflexivity.
-Qed.
-
-Lemma follow_nil
-  {a: p4automaton}
-  (c: configuration a)
-:
-  follow c nil = c
-.
-Proof.
-  reflexivity.
-Qed.
-
-Lemma follow_with_space
-  {a: p4automaton}
-  (s: states a)
-  (st: store a)
-  (buf buf': list bool)
-  (b: bool)
-:
-  length buf + 1 < size a s ->
-  follow (inl s, st, buf) (b :: buf') =
-  follow (inl s, st, buf ++ b :: nil) buf'
-.
-Proof.
-  intros.
-  rewrite follow_cons.
-  f_equal.
-  now apply step_with_space.
-Qed.
+  : configuration a := {
+  follow c nil := c;
+  follow c (b :: input) := follow (step c b) input
+}.
 
 Definition accepting
   {a: p4automaton}
   (c: configuration a)
   : Prop
 :=
-  fst (fst c) = inr true
+  conf_state _ c = inr true
 .
 
 Definition accepted
@@ -140,85 +139,3 @@ Definition lang_equiv
 .
 
 Definition rel a1 a2 := configuration a1 -> configuration a2 -> Prop.
-Definition min_step
-  {a: p4automaton}
-  (c: configuration a)
-:=
-  match c with
-  | (inl s, _, buf) =>
-    max (size a s - length buf) 1
-  | (inr _, _, _) =>
-    1
-  end
-.
-
-Lemma follow_buffer
-  {a: p4automaton}
-  (s: states a)
-  (st: store a)
-  (buf buf': list bool)
-:
-  Datatypes.length buf + Datatypes.length buf' + 1 < size a s ->
-  follow (inl s, st, buf) buf' =
-  (inl s, st, buf ++ buf')
-.
-Proof.
-  induction buf' using rev_ind; intros.
-  - now rewrite follow_nil, app_nil_r.
-  - unfold follow.
-    rewrite fold_left_app.
-    fold (follow (inl s, st, buf) buf').
-    simpl fold_left.
-    rewrite IHbuf'.
-    + rewrite step_with_space.
-      * now rewrite app_assoc.
-      * rewrite app_length in *.
-        simpl in *.
-        lia.
-    + rewrite app_length in *.
-      simpl Datatypes.length in *.
-      lia.
-Qed.
-
-Lemma follow_exact
-  {a: p4automaton}
-  (s: states a)
-  (st: store a)
-  (buf buf': list bool)
-:
-  Datatypes.length buf' > 0 ->
-  Datatypes.length buf + Datatypes.length buf' = size a s ->
-  follow (inl s, st, buf) buf' =
-    let st' := update a s (buf ++ buf') st in
-    (transitions a s st', st', nil)
-.
-Proof.
-  intros.
-  destruct buf'.
-  - simpl Datatypes.length in H.
-    lia.
-  - revert s st buf b H H0.
-    induction buf'; intros.
-    + rewrite follow_cons, follow_nil.
-      unfold step.
-      rewrite app_length.
-      simpl Datatypes.length in *.
-      destruct (equiv_dec _ _); trivial.
-      exfalso; eapply c; auto.
-      
-    + rewrite follow_cons.
-      rewrite step_with_space.
-      rewrite IHbuf'.
-      * repeat f_equal;
-        rewrite <- app_assoc;
-        rewrite <- app_comm_cons;
-        rewrite app_nil_l;
-        easy.
-      * simpl Datatypes.length in *.
-        lia.
-      * rewrite app_length in *.
-        simpl Datatypes.length in *.
-        lia.
-      * simpl Datatypes.length in *.
-        lia.
-Qed.
