deps/poulet4/lib/P4automata/Ntuple.v
@@ -1,0 +1,57 @@
+Require Import Coq.Lists.List.
+Require Import Coq.Classes.EquivDec.
+
+Import ListNotations.
+
+Fixpoint n_tuple A (n: nat): Type :=
+  match n with
+  | 0 => unit
+  | S n => n_tuple A n * A
+  end.
+
+Fixpoint n_tuple_app {A n} (xs: n_tuple A n) (x: A) : n_tuple A (n + 1) :=
+  match n as n' return (n_tuple A n' -> n_tuple A (n' + 1)) with
+  | 0 =>
+    fun _ => (tt, x)
+  | S n =>
+    fun '(xs, x') => (n_tuple_app xs x, x')
+  end xs.
+
+Fixpoint t2l A (n: nat) (x: n_tuple A n) : list A :=
+  match n as n' return n_tuple A n' -> list A with
+  | 0 => fun _ => nil
+  | S n => fun p => t2l A n (fst p) ++ [snd p]
+  end x.
+
+Fixpoint n_tuple_concat' {A n m} (xs: n_tuple A n) (ys: n_tuple A m) : n_tuple A (m + n) :=
+  match m as m' return (n_tuple A m' -> n_tuple A (m' + n)) with
+  | 0 =>
+    fun _ => xs
+  | S m0 =>
+    fun '(ys, y) => (n_tuple_concat' xs ys, y)
+  end ys.
+
+Fixpoint n_tuple_repeat {A: Type} (n: nat) (a: A) : n_tuple A n :=
+  match n with
+  | 0 => tt
+  | S n => ((n_tuple_repeat n a), a)
+  end.
+
+Definition n_tuple_concat {A n m} (xs: n_tuple A n) (ys: n_tuple A m) : n_tuple A (n + m).
+  rewrite Plus.plus_comm.
+  exact (n_tuple_concat' xs ys).
+Defined.
+
+Program Instance n_tuple_eq_dec
+         {A: Type}
+         `{A_eq_dec: EquivDec.EqDec A eq}
+         (n: nat) : EquivDec.EqDec (n_tuple A n) eq.
+Next Obligation.
+Admitted.
+
+Definition n_tuple_take_n {A m} (n: nat) (xs: n_tuple A m) : n_tuple A (Nat.min n m).
+Admitted.
+Definition n_tuple_skip_n {A m} (n: nat) (xs: n_tuple A m) : n_tuple A (m - n).
+Admitted.
+Definition n_tuple_slice {A n} (hi lo: nat) (xs: n_tuple A n) : n_tuple A (1 + hi - lo).
+Admitted.
